extract.zsh
@@ -8,7 +8,7 @@ coq_makefile -f _CoqProject -o Makefile
 make
 
 # Step 3: Add "open Complex" at the beginning of "../qasm/lib/quantum_core.ml"
-sed -i '' '1s/^/open Complex\n/' ../qasm/lib/quantum_core.ml
+sed -i '' '1s/^/open Complex\n/' ../qasm/lib/core/quantum_core.ml
 
 # Step 4: Leave the "core" directory
 cd ..
